

5.6 Q-Learning

Saturday, February 13, 2021

1:52 PM

Q-learning directly updates estimates of Q-factors associated with an optimal policy.

Let us define the optimal Q-factor,

$$Q^*(i, u) = \sum_{j=0}^n p_{ij}(u) (g(i, u, j) + J^*(j)) \quad , \quad i=1, 2, \dots, n$$

$$J^*(i) = \min_{u \in U(i)} Q^*(i, u)$$

Combining the above two, we get,

$$Q^*(i, u) = \sum_{j=0}^n p_{ij}(u) (g(i, u, j) + \min_{v \in U(j)} Q^*(j, v)).$$

Using the uniqueness of Bellman's eq.,

$$\min_{u \in U(i)} Q(i, u) = \min_{u \in U(i)} Q^*(i, u).$$

In terms of Q factors,

$$Q(i, u) = \sum_{j=0}^n p_{ij}(u) (g(i, u, j) + \min_{v \in U(j)} Q(j, v)).$$

More generally,

$$Q(i, u) = (1-\gamma)Q(i, u) + \gamma \sum_{j=0}^n p_{ij}(u) (g(i, u, j) + \min_{v \in U(j)} Q(j, v)).$$

Q-learning is an approximate version of the above update where the expectation is replaced by a single sample,

$$Q(i, u) = (1-\gamma)Q(i, u) + \gamma (g(i, u, j) + \min_{v \in U(j)} Q(j, v)).$$

The Convergence of Q-Learning -

We first write a general statement,

$$Q_{t+1}(i, u) = (1-\gamma_t(i, u)) Q_t(i, u) + \gamma_t(i, u) (g(i, u, j) + \min_{v \in U(j)} Q_t(j, v))$$

$$\gamma_t(i, u) = 0 \text{ for } t \notin T^{iu} \text{ and } Q_t(0, u) = 0 \quad \forall t$$

Proposition-5: Suppose that -

$$\sum_{t=0}^{\infty} \gamma_t(i, u) = \infty, \quad \sum_{t=0}^{\infty} \gamma_t^2(i, u) < \infty, \quad \forall i, u \in U(i)$$

Then $Q_t(i, u)$ converges to $Q^*(i, u)$ with probability 1 in each of the following cases -

(a) If all policies are proper.

(b) If Assumptions 1 and 2 hold and if $Q_t(i, u)$ is bounded with probability 1.

Proof: Consider a mapping H ,

$$H(Q)(i, u) = \sum_{j=0}^n p_{ij}(u) (g(i, u, j) + \min_{v \in U(j)} Q(j, v)),$$

Then Q-learning is of the form,

$$Q_{t+1}(i, u) = (1-\gamma_t(i, u)) Q_t(i, u) + \gamma_t(i, u) (H(Q)(i, u) + u_t(i, u)).$$

$$\text{where } u_t(i, u) = g(i, u, j) + \min_{v \in U(j)} Q_t(j, v) - \sum_{j=0}^n p_{ij}(u) (g(i, u, j) + \min_{v \in U(j)} Q_t(j, v)).$$

Note that $E[u_t(i, u) | F_t] = 0$ and $E[u_t^2(i, u) | F_t] \leq K(1 + \max_{j,v} Q_t^2(j, v))$.

(a) We first consider the case when all policies are proper,

According to Chapter-2 there exist $\xi(i) > 0, i \neq 0$, and a scalar $\beta \in (0, 1)$,

$$\sum_{j=1}^n p_{ij}(u) \xi(j) \leq \beta \xi(i) \quad , \quad \forall i, u \in U(i).$$

For any two vectors Q and \bar{Q} ,

$$\begin{aligned} |H(Q)(i, u) - H(\bar{Q})(i, u)| &\leq \sum_{j=1}^n p_{ij}(u) \left| \min_{v \in U(j)} Q(j, v) - \min_{v \in U(j)} \bar{Q}(j, v) \right|, \\ &\leq \sum_{j=1}^n p_{ij}(u) \max_{v \in U(j)} |Q(j, v) - \bar{Q}(j, v)|, \\ &\leq \sum_{j=1}^n p_{ij}(u) \|Q - \bar{Q}\|_{\infty} \xi(j), \\ &\leq \beta \|Q - \bar{Q}\|_{\infty} \xi(i). \end{aligned}$$

Dividing both sides by $\xi(i)$ and taking min over $\forall i$ and $u \in U(i)$,

$$\|H(Q) - H(\bar{Q})\|_{\infty} \leq \beta \|Q - \bar{Q}\|_{\infty}$$

\therefore , H is a weighted max norm contraction
Convergence of Q-learning follows from Proposition-4 of Chapter-4.

(b) In the second case, we impose assumptions 1 and 2 and remove the case of all proper policies,

Clearly H is a monotone mapping,

$$Q \leq \bar{Q} \Rightarrow H(Q) \leq H(\bar{Q}),$$

Also, for γ a positive scalar and \mathbf{e} being a vector of all components equal to 1,

$$H(Q - \gamma \mathbf{e}) \leq H(Q) \leq H(Q + \gamma \mathbf{e}) \leq H(Q) + \gamma \mathbf{e}.$$

Finally, $H(Q) = Q$ has a unique solution and Q_t converges to Q^* with probability 1 based on Proposition-6 from Chapter 4.

Q-Learning for Discounted Problems.

We may not convert the discounted problem to a stochastic shortest path problem. This can be handled directly,

$$Q(i, u) = (1-\gamma)Q(i, u) + \gamma (g(i, u, j) + \alpha \min_{v \in U(j)} Q(j, v)).$$

Here, α is the discount factor.

Similar convergence results are observed as for the stochastic shortest-path case.